update mkParseTable completeness proofs

Proofs/mkParseTable_correct.v
@@ -11,564 +11,680 @@ Module GeneratorProofsFn (Import G : Grammar.T).
 
   Module Export EntryProofs := EntryProofsFn G.
 
-Definition table_correct_wrt_entries (tbl : parse_table) (es : list table_entry) :=
-  forall x la xp,
-    pt_lookup x la tbl = Some xp
-    <-> x = (lhs xp) /\ In (xp, la) es.
+  Definition table_correct_wrt_entries (tbl : parse_table) (es : list table_entry) :=
+    forall x la xp,
+      pt_lookup x la tbl = Some xp
+      <-> x = (lhs xp) /\ In (xp, la) es.
 
-Lemma invariant_iff_parse_table_correct :
-  forall (g : grammar) (es : list table_entry) (tbl : parse_table),
-    entries_correct es g
-    -> table_correct_wrt_entries tbl es
-       <-> parse_table_correct tbl g.
-Proof.
-  intros g es tbl Hwf.
-  unfold entries_correct in Hwf.
-  split.
-  - intros Htc.
-    unfold table_correct_wrt_entries in Htc.
+  Lemma invariant_iff_parse_table_correct :
+    forall (g : grammar) (es : list table_entry) (tbl : parse_table),
+      entries_correct es g
+      -> table_correct_wrt_entries tbl es
+         <-> parse_table_correct tbl g.
+  Proof.
+    intros g es tbl Hwf.
+    unfold entries_correct in Hwf.
     split.
-    + unfold pt_sound.
-      intros x x' la gamma f Hlk.
-      apply Htc in Hlk; destruct Hlk as [Heq Hin]; subst; simpl in *.
-      split; [auto | apply Hwf; auto].
-    + unfold pt_complete.
-      intros x la gamma f Hin Hlf.
-      apply Htc; simpl.
-      split; [auto | apply Hwf; auto].
-  - intros Hpt.
-    destruct Hpt as [Hsou Hcom].
-    unfold table_correct_wrt_entries.
-    intros x la [(x', gamma) f].
-    split.
-    + intros Hlk.
-      apply Hsou in Hlk; destruct Hlk as [Heq [Hin Hlk]]; subst; simpl in *.
-      split; [auto | apply Hwf; auto].
-    + intros [Heq Hin]; subst; simpl in *.
-      apply Hwf in Hin.
-      destruct Hin as [Hin Hlf].
-      apply Hcom; auto.
-Qed.
-
-(* mkParseTable soundness *)
-
-Lemma addEntry_outer_Some_inner_Some :
-  forall e o tbl,
-    addEntry e o = Some tbl
-    -> exists tbl',
-      o = Some tbl'.
-Proof.
-  intros e o tbl Hadd.
-  unfold addEntry in Hadd.
-  destruct o as [tbl' |] eqn:Ho; tc; subst.
-  dm; dm; tc.
-  inv Hadd; eauto.
-Qed.
-
-Lemma duplicate_preserves_invariant :
-  forall tbl es x la xp,
-    table_correct_wrt_entries tbl es
-    -> pt_lookup x la tbl = Some xp
-    -> table_correct_wrt_entries tbl ((xp, la) :: es).
-Proof.
-  intros tbl es x la xp Htc Hlk.
-  unfold table_correct_wrt_entries.
-  intros x' la' xp'.
-  split.
-  - intros Hlk'.
-    unfold table_correct_wrt_entries in Htc.
-    apply Htc in Hlk'; destruct Hlk' as [Heq Hin]; split; auto.
-    right; auto.
-  - intros [Heq Hin]; subst.
-    unfold table_correct_wrt_entries in Htc.
-    inv Hin.
-    + inv H; auto.
-      pose proof Hlk as Hlk'.
-      apply Htc in Hlk; destruct Hlk as [Heq Hin]; subst; auto.
-    + apply Htc; auto.
-Qed.
-
-Lemma lookup_add_or :
-  forall x x' la la' xp xp' tbl,
-    pt_lookup x' la' (pt_add x la xp tbl) = Some xp'
-    -> (x = x' /\ la = la' /\ xp = xp')
-       \/ pt_lookup x' la' tbl = Some xp'.
-Proof.
-  intros x x' la la' xp xp' tbl Hlk.
-  unfold pt_lookup in Hlk; unfold pt_add in Hlk.
-  rewrite ParseTableFacts.add_o in Hlk.
-  destruct (ParseTableFacts.eq_dec (x, la) (x', la')); auto.
-  inv e; inv Hlk; auto.
-Qed.
-
-Lemma new_entry_preserves_invariant :
-  forall tbl es xp la,
-    table_correct_wrt_entries tbl es
-    -> pt_lookup (lhs xp) la tbl = None
-    -> table_correct_wrt_entries (pt_add (lhs xp) la xp tbl) ((xp, la) :: es).
-Proof.
-  intros tbl es xp la Htc Hlk.
-  unfold table_correct_wrt_entries.
-  intros x' la' xp'.
-  split.
-  - intros Hlk'.
-    apply lookup_add_or in Hlk'.
-    inv Hlk'.
-    + destruct H as [Hx [Hla Hgamma]]; subst; split; auto.
-      left; auto.
-    + apply Htc in H; destruct H as [Heq Hin]; subst; split; auto.
-      right; auto.
-  - intros [Heq Hin]; subst; inv Hin.
-    + inv H.
-      unfold pt_lookup.
-      unfold pt_add.
-      apply ParseTableFacts.add_eq_o; auto.
-    + destruct (ParseTableFacts.eq_dec (lhs xp, la) (lhs xp', la')).
-      * inv e.
-        assert (Hand : lhs xp = lhs xp' /\ In (xp', la') es) by auto.
-        apply Htc in Hand; tc.
-      * unfold pt_lookup.
-        unfold pt_add.
-        rewrite ParseTableFacts.add_neq_o; auto.
-        apply Htc; auto.
-Qed.
-
-(* THIS IS NEW *)
-Definition unique_productions g : Prop :=
-  NoDup (prodsOf g).
-
-Definition unique_action_per_prod (es : list table_entry) : Prop :=
-  forall p f f' la,
-    In (existT _ p f, la) es
-    -> In (existT _ p f', la) es
-    -> f = f'.
-
-Lemma xp_in_xps_impl_p_in_prodOf_xps :
-  forall p f xps,
-    In (existT _ p f) xps -> In p (map prodOf xps).
-Proof.
-  intros p f xps.
-  induction xps as [| (p', f') xps IH]; intros Hin; simpl in *; tc.
-  destruct Hin as [Heq | Hin]; auto.
-  apply EqdepFacts.eq_sigT_fst in Heq; auto.
-Qed.
-
-Lemma unique_productions_unique_action_per_prod' :
-  forall (xps : list xprod)
-         (p : production)
-         (f f' : action_ty p),
-    NoDup (map prodOf xps)
-    -> In (existT _ p f)  xps
-    -> In (existT _ p f') xps
-    -> f = f'.
-Proof.
-  intros xps.
-  induction xps as [| xp xps IH]; intros p f f' Hnd Hin Hin'; simpl in *.
-  - inv Hin.
-  - inv Hnd.
-    destruct Hin as [Heq | Hin]; destruct Hin' as [Heq' | Hin']; subst; simpl in *; auto.
-    + apply Eqdep_dec.inj_pair2_eq_dec; auto.
-      apply production_eq_dec.
-    + apply xp_in_xps_impl_p_in_prodOf_xps in Hin'; tc.
-    + apply xp_in_xps_impl_p_in_prodOf_xps in Hin ; tc.
-Qed.
-
-Lemma unique_productions_unique_action_per_prod :
-  forall g es,
-    unique_productions g
-    -> entries_correct es g
-    -> unique_action_per_prod es.
-Proof.
-  intros g es Hu Hc.
-  unfold unique_action_per_prod.
-  intros p f f' la Hin Hin'.
-  apply Hc in Hin ; destruct Hin  as [Hin _].
-  apply Hc in Hin'; destruct Hin' as [Hin' _].
-  eapply unique_productions_unique_action_per_prod'; eauto.
-Qed.
-
-Lemma addEntry_preserves_invariant :
-  forall (e : table_entry)
-         (es : list table_entry)
-         (tbl' tbl : parse_table),
-    table_correct_wrt_entries tbl' es
-    -> addEntry e (Some tbl') = Some tbl
-    -> unique_action_per_prod (e :: es)
-    -> table_correct_wrt_entries tbl (e :: es).
-Proof.
-  intros e es tbl' tbl Htc Hadd Hu.
-  destruct e as (xp, la) eqn:He.
-  unfold addEntry in Hadd.
-  destruct xp as [(x, gamma) f].
-  destruct (pt_lookup x la tbl') as [[(x', gamma') f'] |] eqn:Hlk.
-  - destruct (Gen.L.production_eq_dec (x, gamma) (x', gamma')) as [Heq | Hneq].
-    + inv Heq; inv Hadd.
-      assert (f = f').
-      { eapply Hu.
-        - left; eauto.
-        - apply Htc in Hlk; destruct Hlk as [Heq Hin].
-          right; auto. }
-      subst.
-      eapply duplicate_preserves_invariant; eauto.
-    + inv Hadd.
-  - inv Hadd.
-    apply new_entry_preserves_invariant with
-        (xp := existT _ (x, gamma) f); auto.
-Qed.
-
-Lemma empty_table_correct_wrt_empty_entries :
-  table_correct_wrt_entries empty_table [].
-Proof.
-  unfold table_correct_wrt_entries.
-  intros x gamma la.
-  split.
-  - intros Hlk.
-    unfold pt_lookup in Hlk.
-    rewrite ParseTableFacts.empty_o in Hlk; inv Hlk.
-  - intros [Heq Hin]; inv Hin.
-Qed.
-
-Lemma unique_action_per_prod_tl :
-  forall e es,
-    unique_action_per_prod (e :: es)
-    -> unique_action_per_prod es.
-Proof.
-  intros e es Hu.
-  unfold unique_action_per_prod.
-  intros p f f' la Hin Hin'.
-  eapply Hu; right; eauto.
-Qed.
-
-Lemma mkParseTable_sound_wrt_invariant :
-  forall (es  : list table_entry)
-         (tbl : parse_table),
-    unique_action_per_prod es
-    -> mkParseTable es = Some tbl
-    -> table_correct_wrt_entries tbl es.
-Proof.
-  intros es.
-  induction es as [| e es]; intros tbl Hu Hmk; simpl in *.
-  - inv Hmk.
-    apply empty_table_correct_wrt_empty_entries.
-  - pose proof Hmk as Hmk'.
-    apply addEntry_outer_Some_inner_Some in Hmk.
-    destruct Hmk as [tbl' Hmk].
-    rewrite Hmk in Hmk'.
-    pose proof Hu as Hu'; apply unique_action_per_prod_tl in Hu.
-    eapply addEntry_preserves_invariant; eauto.
-Qed.
-
-Lemma mkParseTable_sound :
-  forall (es  : list table_entry)
-         (g   : grammar)
-         (tbl : parse_table),
-    unique_action_per_prod es
-    -> entries_correct es g
-    -> mkParseTable es = Some tbl
-    -> parse_table_correct tbl g.
-Proof.
-  intros es g tbl Hua Hwf Hmk.
-  eapply invariant_iff_parse_table_correct; eauto.
-  apply mkParseTable_sound_wrt_invariant; auto.
-Qed.
-
-(* mkParseTable completeness *)
-
-Lemma table_correct_wrt_empty_entries_eq_empty_table :
-  forall tbl,
-    table_correct_wrt_entries tbl []
-    -> ParseTable.Equal tbl empty_table.
-Proof.
-  intros tbl Htc.
-  unfold ParseTable.Equal.
-  intros (x, la).
-  unfold table_correct_wrt_entries in Htc.
-  destruct (pt_lookup x la tbl) as [gamma |] eqn:Hlk.
-  - apply Htc in Hlk.
-    inv Hlk.
-  - rewrite ParseTableFacts.empty_o; auto.
-Qed.
-
-Lemma invariant_cons_duplicate_invariant_tail :
-  forall tbl x gamma la ps,
-    table_correct_wrt_entries tbl ((x, la, gamma) :: ps)
-    -> In (x, la, gamma) ps
-    -> table_correct_wrt_entries tbl ps.
-Proof.
-  intros tbl x gamma la es Htc Hin.
-  unfold table_correct_wrt_entries in Htc.
-  unfold table_correct_wrt_entries.
-  intros x' gamma' la'.
-  split.
-  - intros Hlk.
-    apply Htc in Hlk.
-    inv Hlk; auto.
-    inv H; auto.
-  - intros Hin'.
-    apply Htc.
-    right; auto.
-Qed.
-
-Lemma eq_pairs_eq_gammas :
-  forall tbl es x gamma gamma' la,
-    table_correct_wrt_entries tbl es
-    -> In (x, la, gamma) es
-    -> In (x, la, gamma') es
-    -> gamma = gamma'.
-Proof.
-  intros tbl es x gamma gamma' la Htc Hin Hin'.
-  apply Htc in Hin.
-  apply Htc in Hin'.
-  congruence.
-Qed.
-  
-Lemma invariant_cons_eq_gammas :
-  forall tbl x gamma la es,
-    table_correct_wrt_entries tbl ((x, la, gamma) :: es)
-    -> forall gamma',
-      In (x, la, gamma') es
-      -> gamma = gamma'.
-Proof.
-  intros tbl x gamma la es Htc gamma' Hin.
-  unfold table_correct_wrt_entries in Htc.
-  destruct (list_eq_dec symbol_eq_dec gamma gamma'); auto.
-  assert (H : In (x, la, gamma) ((x, la, gamma) :: es)).
-  { left; auto. }
-  assert (H' : In (x, la, gamma') ((x, la, gamma) :: es)).
-  { right; auto. }
-  apply Htc in H.
-  apply Htc in H'.
-  congruence.
-Qed.
-  
-(* BUG : originally had this as add instead of remove *)
-Lemma invariant_cons_new_entry_invariant_remove :
-  forall tbl x gamma la ps,
-    table_correct_wrt_entries tbl ((x, la, gamma) :: ps)
-    -> ~In (x, la, gamma) ps
-    -> table_correct_wrt_entries (ParseTable.remove (x, la) tbl) ps.
-Proof.
-  intros tbl x gamma la es Htc Hin.
-  unfold table_correct_wrt_entries.
-  intros x' gamma' la'.
-  split.
-  - intros Hlk.
-    destruct (ParseTableFacts.eq_dec (x, la) (x', la')).
-    + inv e.
-      unfold pt_lookup in Hlk.
-      rewrite ParseTableFacts.remove_eq_o in Hlk; inv Hlk; auto.
-    + unfold pt_lookup in Hlk.
-      rewrite ParseTableFacts.remove_neq_o in Hlk; auto.
+    - intros Htc.
       unfold table_correct_wrt_entries in Htc.
-      apply Htc in Hlk.
-      inv Hlk; congruence.
-  - intros Hin'.
-    destruct (ParseTableFacts.eq_dec (x, la) (x', la')).
-    + inv e.
-      destruct (list_eq_dec symbol_eq_dec gamma gamma').
-      * subst.
-        congruence.
-      * eapply invariant_cons_eq_gammas with (gamma' := gamma') in Htc; auto.
-        congruence.
-    + unfold pt_lookup.
-      rewrite ParseTableFacts.remove_neq_o; auto.
+      split.
+      + unfold pt_sound.
+        intros x x' la gamma f Hlk.
+        apply Htc in Hlk; destruct Hlk as [Heq Hin]; subst; simpl in *.
+        split; [auto | apply Hwf; auto].
+      + unfold pt_complete.
+        intros x la gamma f Hin Hlf.
+        apply Htc; simpl.
+        split; [auto | apply Hwf; auto].
+    - intros Hpt.
+      destruct Hpt as [Hsou Hcom].
+      unfold table_correct_wrt_entries.
+      intros x la [(x', gamma) f].
+      split.
+      + intros Hlk.
+        apply Hsou in Hlk; destruct Hlk as [Heq [Hin Hlk]]; subst; simpl in *.
+        split; [auto | apply Hwf; auto].
+      + intros [Heq Hin]; subst; simpl in *.
+        apply Hwf in Hin.
+        destruct Hin as [Hin Hlf].
+        apply Hcom; auto.
+  Qed.
+
+  (* mkParseTable soundness *)
+
+  Lemma addEntry_outer_Some_inner_Some :
+    forall e o tbl,
+      addEntry e o = Some tbl
+      -> exists tbl',
+        o = Some tbl'.
+  Proof.
+    intros e o tbl Hadd.
+    unfold addEntry in Hadd.
+    destruct o as [tbl' |] eqn:Ho; tc; subst.
+    dm; dm; tc.
+    inv Hadd; eauto.
+  Qed.
+
+  Lemma duplicate_preserves_invariant :
+    forall tbl es x la xp,
+      table_correct_wrt_entries tbl es
+      -> pt_lookup x la tbl = Some xp
+      -> table_correct_wrt_entries tbl ((xp, la) :: es).
+  Proof.
+    intros tbl es x la xp Htc Hlk.
+    unfold table_correct_wrt_entries.
+    intros x' la' xp'.
+    split.
+    - intros Hlk'.
+      unfold table_correct_wrt_entries in Htc.
+      apply Htc in Hlk'; destruct Hlk' as [Heq Hin]; split; auto.
+      right; auto.
+    - intros [Heq Hin]; subst.
+      unfold table_correct_wrt_entries in Htc.
+      inv Hin.
+      + inv H; auto.
+        pose proof Hlk as Hlk'.
+        apply Htc in Hlk; destruct Hlk as [Heq Hin]; subst; auto.
+      + apply Htc; auto.
+  Qed.
+
+  Lemma lookup_add_or :
+    forall x x' la la' xp xp' tbl,
+      pt_lookup x' la' (pt_add x la xp tbl) = Some xp'
+      -> (x = x' /\ la = la' /\ xp = xp')
+         \/ pt_lookup x' la' tbl = Some xp'.
+  Proof.
+    intros x x' la la' xp xp' tbl Hlk.
+    unfold pt_lookup in Hlk; unfold pt_add in Hlk.
+    rewrite ParseTableFacts.add_o in Hlk.
+    destruct (ParseTableFacts.eq_dec (x, la) (x', la')); auto.
+    inv e; inv Hlk; auto.
+  Qed.
+
+  Lemma new_entry_preserves_invariant :
+    forall tbl es xp la,
+      table_correct_wrt_entries tbl es
+      -> pt_lookup (lhs xp) la tbl = None
+      -> table_correct_wrt_entries (pt_add (lhs xp) la xp tbl) ((xp, la) :: es).
+  Proof.
+    intros tbl es xp la Htc Hlk.
+    unfold table_correct_wrt_entries.
+    intros x' la' xp'.
+    split.
+    - intros Hlk'.
+      apply lookup_add_or in Hlk'.
+      inv Hlk'.
+      + destruct H as [Hx [Hla Hgamma]]; subst; split; auto.
+        left; auto.
+      + apply Htc in H; destruct H as [Heq Hin]; subst; split; auto.
+        right; auto.
+    - intros [Heq Hin]; subst; inv Hin.
+      + inv H.
+        unfold pt_lookup.
+        unfold pt_add.
+        apply ParseTableFacts.add_eq_o; auto.
+      + destruct (ParseTableFacts.eq_dec (lhs xp, la) (lhs xp', la')).
+        * inv e.
+          assert (Hand : lhs xp = lhs xp' /\ In (xp', la') es) by auto.
+          apply Htc in Hand; tc.
+        * unfold pt_lookup.
+          unfold pt_add.
+          rewrite ParseTableFacts.add_neq_o; auto.
+          apply Htc; auto.
+  Qed.
+
+  (* THIS IS NEW *)
+  Definition unique_productions g : Prop :=
+    NoDup (prodsOf g).
+
+  Definition unique_action_per_prod (es : list table_entry) : Prop :=
+    forall p f f' la,
+      In (existT _ p f, la) es
+      -> In (existT _ p f', la) es
+      -> f = f'.
+
+  Lemma xp_in_xps_impl_p_in_prodOf_xps :
+    forall p f xps,
+      In (existT _ p f) xps -> In p (map prodOf xps).
+  Proof.
+    intros p f xps Hin.
+    eapply in_map with (f := prodOf) in Hin; auto.
+  Qed.
+
+  Lemma unique_productions_unique_action_per_prod' :
+    forall (xps : list xprod)
+           (p : production)
+           (f f' : action_ty p),
+      NoDup (map prodOf xps)
+      -> In (existT _ p f)  xps
+      -> In (existT _ p f') xps
+      -> f = f'.
+  Proof.
+    intros xps.
+    induction xps as [| xp xps IH]; intros p f f' Hnd Hin Hin'; simpl in *.
+    - inv Hin.
+    - inv Hnd.
+      destruct Hin as [Heq | Hin]; destruct Hin' as [Heq' | Hin']; subst; simpl in *; auto.
+      + apply Eqdep_dec.inj_pair2_eq_dec; auto.
+        apply production_eq_dec.
+      + apply xp_in_xps_impl_p_in_prodOf_xps in Hin'; tc.
+      + apply xp_in_xps_impl_p_in_prodOf_xps in Hin ; tc.
+  Qed.
+
+  Lemma unique_productions_unique_action_per_prod :
+    forall g es,
+      unique_productions g
+      -> entries_correct es g
+      -> unique_action_per_prod es.
+  Proof.
+    intros g es Hu Hc.
+    unfold unique_action_per_prod.
+    intros p f f' la Hin Hin'.
+    apply Hc in Hin ; destruct Hin  as [Hin _].
+    apply Hc in Hin'; destruct Hin' as [Hin' _].
+    eapply unique_productions_unique_action_per_prod'; eauto.
+  Qed.
+
+  Lemma addEntry_preserves_invariant :
+    forall (e : table_entry)
+           (es : list table_entry)
+           (tbl' tbl : parse_table),
+      table_correct_wrt_entries tbl' es
+      -> addEntry e (Some tbl') = Some tbl
+      -> unique_action_per_prod (e :: es)
+      -> table_correct_wrt_entries tbl (e :: es).
+  Proof.
+    intros e es tbl' tbl Htc Hadd Hu.
+    destruct e as (xp, la) eqn:He.
+    unfold addEntry in Hadd.
+    destruct xp as [(x, gamma) f].
+    destruct (pt_lookup x la tbl') as [[(x', gamma') f'] |] eqn:Hlk.
+    - destruct (Gen.L.production_eq_dec (x, gamma) (x', gamma')) as [Heq | Hneq].
+      + inv Heq; inv Hadd.
+        assert (f = f').
+        { eapply Hu.
+          - left; eauto.
+          - apply Htc in Hlk; destruct Hlk as [Heq Hin].
+            right; auto. }
+        subst.
+        eapply duplicate_preserves_invariant; eauto.
+      + inv Hadd.
+    - inv Hadd.
+      apply new_entry_preserves_invariant with
+          (xp := existT _ (x, gamma) f); auto.
+  Qed.
+
+  Lemma empty_table_correct_wrt_empty_entries :
+    table_correct_wrt_entries empty_table [].
+  Proof.
+    unfold table_correct_wrt_entries.
+    intros x gamma la.
+    split.
+    - intros Hlk.
+      unfold pt_lookup in Hlk.
+      rewrite ParseTableFacts.empty_o in Hlk; inv Hlk.
+    - intros [Heq Hin]; inv Hin.
+  Qed.
+
+  Lemma unique_action_per_prod_tl :
+    forall e es,
+      unique_action_per_prod (e :: es)
+      -> unique_action_per_prod es.
+  Proof.
+    intros e es Hu.
+    unfold unique_action_per_prod.
+    intros p f f' la Hin Hin'.
+    eapply Hu; right; eauto.
+  Qed.
+
+  Lemma mkParseTable_sound_wrt_invariant :
+    forall (es  : list table_entry)
+           (tbl : parse_table),
+      unique_action_per_prod es
+      -> mkParseTable es = Some tbl
+      -> table_correct_wrt_entries tbl es.
+  Proof.
+    intros es.
+    induction es as [| e es]; intros tbl Hu Hmk; simpl in *.
+    - inv Hmk.
+      apply empty_table_correct_wrt_empty_entries.
+    - pose proof Hmk as Hmk'.
+      apply addEntry_outer_Some_inner_Some in Hmk.
+      destruct Hmk as [tbl' Hmk].
+      rewrite Hmk in Hmk'.
+      pose proof Hu as Hu'; apply unique_action_per_prod_tl in Hu.
+      eapply addEntry_preserves_invariant; eauto.
+  Qed.
+
+  Lemma mkParseTable_sound :
+    forall (es  : list table_entry)
+           (g   : grammar)
+           (tbl : parse_table),
+      unique_action_per_prod es
+      -> entries_correct es g
+      -> mkParseTable es = Some tbl
+      -> parse_table_correct tbl g.
+  Proof.
+    intros es g tbl Hua Hwf Hmk.
+    eapply invariant_iff_parse_table_correct; eauto.
+    apply mkParseTable_sound_wrt_invariant; auto.
+  Qed.
+
+  (* mkParseTable completeness *)
+
+  Lemma table_correct_wrt_empty_entries_eq_empty_table :
+    forall tbl,
+      table_correct_wrt_entries tbl []
+      -> ParseTable.Equal tbl empty_table.
+  Proof.
+    intros tbl Htc.
+    unfold ParseTable.Equal.
+    intros (x, la).
+    unfold table_correct_wrt_entries in Htc.
+    destruct (pt_lookup x la tbl) as [gamma |] eqn:Hlk.
+    - apply Htc in Hlk; destruct Hlk as [Heq Hin].
+      inv Hin.
+    - rewrite ParseTableFacts.empty_o; auto.
+  Qed.
+
+  Lemma invariant_cons_duplicate_invariant_tail :
+    forall tbl xp la es,
+      table_correct_wrt_entries tbl ((xp, la) :: es)
+      -> In (xp, la) es
+      -> table_correct_wrt_entries tbl es.
+  Proof.
+    intros tbl xp la es Htc Hin.
+    unfold table_correct_wrt_entries.
+    intros x la' xp'.
+    split.
+    - intros Hlk.
+      apply Htc in Hlk; destruct Hlk as [Heq Hin']; subst.
+      split; auto.
+      destruct Hin' as [Heq | Hin']; auto.
+      inv Heq; auto.
+    - intros [Heq Hin']; subst.
       apply Htc.
-      right; auto.
-Qed.
-    
-Lemma correct_post_table_implies_correct_pre_table :
-  forall tbl x gamma la es,
-    table_correct_wrt_entries tbl ((x, la, gamma) :: es)
-    -> exists tbl',
-      table_correct_wrt_entries tbl' es.
-Proof.
-  intros tbl x gamma la es Htc.
-  destruct (in_dec table_entry_dec (x, la, gamma) es).
-  - (* duplicate *)
-    exists tbl.
-    eapply invariant_cons_duplicate_invariant_tail; eauto.
-  - exists (ParseTable.remove (x, la) tbl).
-    eapply invariant_cons_new_entry_invariant_remove; eauto.
-Qed.
+      split; [auto | right; auto].
+  Qed.
 
-Lemma invariant_tables_eq :
-  forall tbl tbl' ps,
-    table_correct_wrt_entries tbl ps
-    -> table_correct_wrt_entries tbl' ps
-    -> ParseTable.Equal tbl tbl'.
-Proof.
-  intros tbl tbl' es Htc Htc'.
-  unfold ParseTable.Equal.
-  intros (x, la).
-  destruct (ParseTable.find (x, la) tbl) as [gamma |] eqn:Hf.
-  - destruct (ParseTable.find (x, la) tbl') as [gamma' |] eqn:Hf'.
-    + apply Htc in Hf.
-      apply Htc' in Hf'.
-      eapply eq_pairs_eq_gammas with
-          (gamma := gamma)
-          (gamma' := gamma') in Htc; eauto.
-      congruence.
-    + apply Htc in Hf.
-      apply Htc' in Hf.
-      unfold pt_lookup in Hf; congruence.
-  - destruct (ParseTable.find (x, la) tbl') as [gamma' |] eqn:Hf'.
-    + apply Htc' in Hf'.
-      apply Htc in Hf'.
-      unfold pt_lookup in Hf'; congruence.
-    + auto.
-Qed.
+  Lemma eq_keys_eq_gammas :
+    forall tbl es xp xp' la,
+      table_correct_wrt_entries tbl es
+      -> In (xp, la) es
+      -> In (xp', la) es
+      -> lhs xp = lhs xp'
+      -> rhs xp = rhs xp'.
+  Proof.
+    intros tbl es xp xp' la Htc Hin Hin' Hl.
+    unfold table_correct_wrt_entries in Htc.
+    assert (Hand : lhs xp = lhs xp
+                   /\ In (xp, la) es) by auto.
+    assert (Hand' : lhs xp = lhs xp'
+                    /\ In (xp', la) es) by auto.
+    apply Htc in Hand; apply Htc in Hand'; tc.
+  Qed.
 
-Lemma invariant_not_in_add :
-  forall tbl tbl' es x gamma la,
-    table_correct_wrt_entries tbl es
-    -> table_correct_wrt_entries tbl' ((x, la, gamma) :: es)
-    -> ~In (x, la, gamma) es
-    -> table_correct_wrt_entries (pt_add x la gamma tbl) ((x, la, gamma) :: es).
-Proof.
-  intros tbl tbl' es x gamma la Htc Htc' Hin.
-  intros x' gamma' la'.
-  split.
-  - intros Hlk.
-    unfold pt_lookup, pt_add in Hlk.
-    destruct (ParseTableFacts.eq_dec (x, la) (x', la')).
-    + inv e.
-      rewrite ParseTableFacts.add_eq_o in Hlk; auto.
-      inv Hlk.
-      left; auto.
-    + rewrite ParseTableFacts.add_neq_o in Hlk; auto.
-      apply Htc in Hlk.
-      right; auto.
-  - intros Hin'.
-    unfold pt_lookup, pt_add.
-    inv Hin'.
-    + inv H.
-      rewrite ParseTableFacts.add_eq_o; auto.
-    + destruct (ParseTableFacts.eq_dec (x, la) (x', la')).
-      * inv e.
-        apply invariant_cons_eq_gammas with (gamma' := gamma') in Htc'; auto.
-        congruence.
-      * rewrite ParseTableFacts.add_neq_o; auto.
-        apply Htc; auto.
-Qed.
+  Lemma invariant_cons_eq_gammas :
+    forall tbl xp xp' la es,
+      table_correct_wrt_entries tbl ((xp, la) :: es)
+      -> In (xp', la) es
+      -> lhs xp = lhs xp'
+      -> rhs xp = rhs xp'.
+  Proof.
+    intros tbl xp xp' la es Htc Hin Hl.
+    unfold table_correct_wrt_entries in Htc.
+    assert (H : lhs xp = lhs xp
+                /\ In (xp, la) ((xp, la) :: es))
+      by (simpl; auto).
+    assert (H' : lhs xp = lhs xp'
+                 /\ In (xp', la) ((xp, la) :: es))
+      by (simpl; auto).
+    apply Htc in H; apply Htc in H'; tc.
+  Qed.
 
-Lemma add_preserves_equal :
-  forall tbl tbl' x la gamma,
-    ParseTable.Equal tbl tbl'
-    -> ParseTable.Equal (pt_add x la gamma tbl) (pt_add x la gamma tbl').
-Proof.
-  intros tbl tbl' x la gamma Heq.
-  unfold ParseTable.Equal.
-  intros (x', la').
-  unfold pt_add.
-  destruct (ParseTableFacts.eq_dec (x, la) (x', la')).
-  - inv e.
-    repeat rewrite ParseTableFacts.add_eq_o; auto.
-  - repeat rewrite ParseTableFacts.add_neq_o; auto.
-Qed.
+  Definition actionOf (xp : xprod) := projT2 xp.
 
-Lemma addEntry_duplicate_doesn't_change_table :
-  forall tbl es x gamma la,
-    table_correct_wrt_entries tbl es
-    -> In (x, la, gamma) es
-    -> addEntry (x, la, gamma) (Some tbl) = Some tbl.
-Proof.
-  intros tbl es x gamma la Htc Hin.
-  unfold addEntry.
-  apply Htc in Hin.
-  rewrite Hin.
-  (* lemma? *)
-  destruct (list_eq_dec symbol_eq_dec gamma gamma); [auto | congruence].
-Qed.
+  Lemma lhs_rhs_eq_uapp_xprods_eq :
+    forall xp xp' la es,
+      lhs xp = lhs xp'
+      -> rhs xp = rhs xp'
+      -> In (xp, la) es
+      -> In (xp', la) es
+      -> unique_action_per_prod es
+      -> xp = xp'.
+  Proof.
+    intros [(x, gamma) f] [(x', gamma') g] la es Hl Hr Hi Hi' Hu; simpl in *; subst.
+    eapply Hu in Hi; eauto.
+    apply Hi in Hi'; subst; auto.
+  Qed.  
+  
+  (* BUG : originally had this as add instead of remove *)
+  Lemma invariant_cons_new_entry_invariant_remove :
+    forall tbl xp la es,
+      unique_action_per_prod ((xp, la) :: es)
+      -> table_correct_wrt_entries tbl ((xp, la) :: es)
+      -> ~In (xp, la) es
+      -> table_correct_wrt_entries (ParseTable.remove (lhs xp, la) tbl) es.
+  Proof.
+    intros tbl xp la es Hu Htc Hin.
+    unfold table_correct_wrt_entries.
+    intros x' la' xp'.
+    split.
+    - intros Hlk.
+      destruct (ParseTableFacts.eq_dec (lhs xp, la) (x', la')).
+      + inv e.
+        unfold pt_lookup in Hlk.
+        rewrite ParseTableFacts.remove_eq_o in Hlk; inv Hlk; auto.
+      + unfold pt_lookup in Hlk.
+        rewrite ParseTableFacts.remove_neq_o in Hlk; auto.
+        unfold table_correct_wrt_entries in Htc.
+        apply Htc in Hlk; destruct Hlk as [Heq Hin']; subst.
+        split; auto.
+        inv Hin'; tc.
+    - intros [Heq Hin']; subst.
+      destruct (ParseTableFacts.eq_dec (lhs xp, la) (lhs xp', la')).
+      + inv e.
+        assert (xp = xp').
+        { eapply lhs_rhs_eq_uapp_xprods_eq with
+              (la := la')
+              (es := ((xp, la') :: es)); eauto.
+          - eapply invariant_cons_eq_gammas in Htc; eauto.
+          - left; auto.
+          - right; auto. }
+        subst; tc.
+      + unfold pt_lookup.
+        rewrite ParseTableFacts.remove_neq_o; auto.
+        apply Htc; split; auto; right; auto.
+  Qed.
 
-Lemma equal_preserves_invariant :
-  forall tbl tbl' ps,
-    table_correct_wrt_entries tbl ps
-    -> ParseTable.Equal tbl tbl'
-    -> table_correct_wrt_entries tbl' ps.
-Proof.
-  intros tbl tbl' es Htc Heq.
-  auto.
-  unfold table_correct_wrt_entries in Htc.
-  unfold pt_lookup in Htc.
-  intros x gamma la.
-  split; [intros Hlk | intros Hin].
-  - apply Htc.
-    unfold ParseTable.Equal in Heq.
-    rewrite Heq; auto.
-  - unfold pt_lookup. 
-    rewrite <- Heq.
-    apply Htc; auto.
-Qed.
+  Definition pl_pair := (production * lookahead)%type.
 
-Lemma addEntry_new_entry_pt_add :
-  forall tbl tbl' es x gamma la,
-    table_correct_wrt_entries tbl es
-    -> table_correct_wrt_entries tbl' ((x, la, gamma) :: es)
-    -> ~ In (x, la, gamma) es
-    -> addEntry (x, la, gamma) (Some tbl) = Some (pt_add x la gamma tbl).
-Proof.
-  intros tbl tbl' es x gamma la Htc Htc' Hin.
-  unfold addEntry.
-  destruct (pt_lookup x la tbl) as [gamma' |] eqn:Hlk.
-  - apply Htc in Hlk. 
-    apply invariant_cons_eq_gammas with (gamma' := gamma') in Htc'; auto.
-    congruence.
-  - auto.
-Qed.
+  Definition plPairOf (e : table_entry) :=
+    match e with
+    | (existT _ p _, la) => (p, la)
+    end.
 
-Lemma mkParseTable_complete_wrt_invariant :
-  forall es tbl,
-    table_correct_wrt_entries tbl es
-    -> exists tbl',
+  Definition plPairsOf (es : list table_entry) :=
+    map plPairOf es.
+
+  Lemma pl_pair_eq_dec :
+    forall p p' : pl_pair,
+      {p = p'} + {p <> p'}.
+  Proof.
+    repeat decide equality.
+  Qed.
+
+  Lemma in_plPairsOf_ex_in_entries :
+    forall p la es,
+      In (p, la) (plPairsOf es)
+      -> exists f,
+        In (existT _ p f, la) es.
+  Proof.
+    intros p la es Hin.
+    unfold plPairsOf in Hin.
+    eapply in_map_iff in Hin.
+    destruct Hin as [e [Heq Hin]].
+    destruct e as [(x, gamma) f]; simpl in *.
+    inv Heq; eauto.
+  Qed.
+
+
+  Lemma not_in_plPairsOf_not_in_entries :
+    forall p f la es,
+      ~ In (p, la) (plPairsOf es)
+      -> ~ In (existT _ p f, la) es.
+  Proof.
+    intros p f la es Hnin; unfold not; intros Hin; apply Hnin.
+    unfold plPairsOf.
+    apply in_map with (f := plPairOf) in Hin; auto.
+  Qed.
+
+  Lemma correct_post_table_implies_correct_pre_table :
+    forall tbl e es,
+      unique_action_per_prod (e :: es)
+      -> table_correct_wrt_entries tbl (e :: es)
+      -> exists tbl',
+          table_correct_wrt_entries tbl' es.
+  Proof.
+    intros tbl e es Hu Htc.
+    destruct (in_dec pl_pair_eq_dec (plPairOf e) (plPairsOf es)); subst; simpl in *.
+    - destruct e as [[p f] la]; simpl in *.
+      apply in_plPairsOf_ex_in_entries in i.
+      destruct i as [g Hin].
+      assert (f = g).
+      { eapply Hu; [left; eauto | right; eauto]. }
+      subst.
+      exists tbl.
+      eapply invariant_cons_duplicate_invariant_tail; eauto.
+    - destruct e as ([(x,gamma) f], la); simpl in *.
+      exists (ParseTable.remove (x, la) tbl).
+      eapply invariant_cons_new_entry_invariant_remove in Htc; eauto.
+      apply not_in_plPairsOf_not_in_entries; auto.
+  Qed.
+
+  Lemma invariant_tables_eq :
+    forall tbl tbl' es,
+      unique_action_per_prod es
+      -> table_correct_wrt_entries tbl es
+      -> table_correct_wrt_entries tbl' es
+      -> ParseTable.Equal tbl tbl'.
+  Proof.
+    intros tbl tbl' es Hu Htc Htc'.
+    unfold ParseTable.Equal.
+    intros (x, la).
+    destruct (ParseTable.find (x, la) tbl) as [xp |] eqn:Hf.
+    - destruct (ParseTable.find (x, la) tbl') as [xp' |] eqn:Hf'.
+      + apply Htc in Hf; destruct Hf as [Heq Hin]; subst.
+        apply Htc' in Hf'; destruct Hf' as [Heq Hin']; subst.
+        assert (xp = xp').
+        { eapply lhs_rhs_eq_uapp_xprods_eq; eauto.
+          eapply eq_keys_eq_gammas; eauto. }
+        subst; auto.
+      + apply Htc in Hf; destruct Hf as [Heq Hin]; subst.
+        unfold table_correct_wrt_entries in Htc'.
+        assert (H : lhs xp = lhs xp /\ In (xp, la) es) by auto.
+        apply Htc' in H.
+        unfold pt_lookup in H; tc.
+    - destruct (ParseTable.find (x, la) tbl') as [xp' |] eqn:Hf'.
+      + apply Htc' in Hf'.
+        apply Htc in Hf'.
+        unfold pt_lookup in Hf'; congruence.
+      + auto.
+  Qed.
+
+  Lemma invariant_not_in_add :
+    forall tbl tbl' es xp la,
+      unique_action_per_prod ((xp, la) :: es)
+      -> table_correct_wrt_entries tbl es
+      -> table_correct_wrt_entries tbl' ((xp, la) :: es)
+      -> ~In (xp, la) es
+      -> table_correct_wrt_entries (pt_add (lhs xp) la xp tbl) ((xp, la) :: es).
+  Proof.
+    intros tbl tbl' es xp la Hu Htc Htc' Hin.
+    intros x' la' xp'.
+    split.
+    - intros Hlk.
+      unfold pt_lookup, pt_add in Hlk.
+      destruct (ParseTableFacts.eq_dec (lhs xp, la) (x', la')).
+      + inv e.
+        rewrite ParseTableFacts.add_eq_o in Hlk; auto.
+        inv Hlk; split; auto; left; auto.
+      + rewrite ParseTableFacts.add_neq_o in Hlk; auto.
+        apply Htc in Hlk; destruct Hlk as [Heq Hin']; subst.
+        split; auto; right; auto.
+    - intros [Heq Hin']; subst.
+      unfold pt_lookup, pt_add.
+      inv Hin'.
+      + inv H.
+        rewrite ParseTableFacts.add_eq_o; auto.
+      + destruct (ParseTableFacts.eq_dec (lhs xp, la) (lhs xp', la')).
+        * inv e.
+          assert (xp = xp').
+          { eapply lhs_rhs_eq_uapp_xprods_eq with
+                (es := (xp, la') :: es); eauto.
+            - eapply eq_keys_eq_gammas; eauto.
+              + left; auto.
+              + right; auto.
+            - left; auto.
+            - right; auto. }
+          subst.
+          apply invariant_cons_eq_gammas with (xp' := xp') in Htc'; auto; tc.
+        * rewrite ParseTableFacts.add_neq_o; auto.
+          apply Htc; auto.
+  Qed.
+
+  Lemma add_preserves_equal :
+    forall tbl tbl' x la xp,
       ParseTable.Equal tbl tbl'
-      /\ mkParseTable es = Some tbl'.
-Proof.
-  intros es.
-  induction es as [| ((x, la), gamma) es]; intros post_tbl Htc.
-  - apply table_correct_wrt_empty_entries_eq_empty_table in Htc.
-    exists empty_table; auto.
-  - pose proof Htc as Htc'.
-    apply correct_post_table_implies_correct_pre_table in Htc.
-    destruct Htc as [pre_tbl Htc].
-    pose proof Htc as Htc''.
-    apply IHes in Htc.
-    destruct Htc as [pre_tbl' [Hpreq Hpremk]].
-    destruct (in_dec table_entry_dec (x, la, gamma) es).
-    + exists pre_tbl'; split.
-      * apply invariant_cons_duplicate_invariant_tail in Htc'; auto.
-        apply ParseTableFacts.Equal_trans with (m' := pre_tbl); auto.
-        eapply invariant_tables_eq; eauto.
-      * simpl.
-        rewrite Hpremk.
-        eapply addEntry_duplicate_doesn't_change_table; eauto.
-        eapply equal_preserves_invariant; eauto.
-    + exists (pt_add x la gamma pre_tbl'); split.
-      * eapply invariant_not_in_add in Htc''; eauto.
-        apply add_preserves_equal with 
-            (x := x)
-            (la := la)
-            (gamma := gamma) in Hpreq; eauto.
-        apply invariant_tables_eq with (tbl := post_tbl) in Htc''; auto.
-        apply ParseTableFacts.Equal_trans with (m' := pt_add x la gamma pre_tbl); auto.
-      * simpl.
-        rewrite Hpremk.
-        eapply addEntry_new_entry_pt_add; eauto.
-        eapply equal_preserves_invariant; eauto.
-Qed.
+      -> ParseTable.Equal (pt_add x la xp tbl) (pt_add x la xp tbl').
+  Proof.
+    intros tbl tbl' x la xp Heq.
+    unfold ParseTable.Equal.
+    intros (x', la').
+    unfold pt_add.
+    destruct (ParseTableFacts.eq_dec (x, la) (x', la')).
+    - inv e.
+      repeat rewrite ParseTableFacts.add_eq_o; auto.
+    - repeat rewrite ParseTableFacts.add_neq_o; auto.
+  Qed.
 
-Lemma mkParseTable_complete :
-  forall (es  : list table_entry)
-         (g   : grammar)
-         (tbl : parse_table),
-    entries_correct es g
-    -> parse_table_correct tbl g
-    -> exists tbl',
-        ParseTable.Equal tbl tbl'
-        /\ mkParseTable es = Some tbl'.
-Proof.
-  intros es g tbl Hwf Hpt.
-  eapply mkParseTable_complete_wrt_invariant.
-  eapply invariant_iff_parse_table_correct; eauto.
-Qed.
+  Lemma addEntry_duplicate_doesn't_change_table :
+    forall tbl es xp la,
+      table_correct_wrt_entries tbl es
+      -> In (xp, la) es
+      -> addEntry (xp, la) (Some tbl) = Some tbl.
+  Proof.
+    intros tbl es xp la Htc Hin.
+    unfold addEntry.
+    destruct xp as [(x, gamma) f].
+    assert (H : x = lhs (existT _ (x, gamma) f)
+                /\ In (existT _ (x, gamma) f, la) es) by auto.
+    apply Htc in H.
+    rewrite H.
+    destruct (Gen.L.production_eq_dec (x, gamma) (x, gamma)); [auto | congruence].
+  Qed.
+
+  Lemma equal_preserves_invariant :
+    forall tbl tbl' ps,
+      table_correct_wrt_entries tbl ps
+      -> ParseTable.Equal tbl tbl'
+      -> table_correct_wrt_entries tbl' ps.
+  Proof.
+    intros tbl tbl' es Htc Heq.
+    auto.
+    unfold table_correct_wrt_entries in Htc.
+    unfold pt_lookup in Htc.
+    intros x gamma la.
+    split; [intros Hlk | intros Hin].
+    - apply Htc.
+      unfold ParseTable.Equal in Heq.
+      rewrite Heq; auto.
+    - unfold pt_lookup. 
+      rewrite <- Heq.
+      apply Htc; auto.
+  Qed.
+
+  Lemma addEntry_new_entry_pt_add :
+    forall tbl tbl' es xp la,
+      unique_action_per_prod ((xp, la) :: es)
+      -> table_correct_wrt_entries tbl es
+      -> table_correct_wrt_entries tbl' ((xp, la) :: es)
+      -> ~ In (xp, la) es
+      -> addEntry (xp, la) (Some tbl) = Some (pt_add (lhs xp) la xp tbl).
+  Proof.
+    intros tbl tbl' es xp la Hu Htc Htc' Hin.
+    destruct (pt_lookup (lhs xp) la tbl) as [xp' |] eqn:Hlk.
+    - assert (xp = xp').
+      (* lemma *)
+      { apply Htc with (x := lhs xp) in Hlk.
+        destruct Hlk as [Heq Hin']; subst.
+        eapply lhs_rhs_eq_uapp_xprods_eq with
+            (es := (xp, la) :: es); eauto.
+        - eapply eq_keys_eq_gammas; eauto.
+          + left; auto.
+          + right; auto.
+        - left; auto.
+        - right; auto. }
+      subst.
+      eapply Htc in Hlk; destruct Hlk as [Heq Hin']; subst; tc.
+    - destruct xp as [(x, gamma) f]; simpl in *.
+      rewrite Hlk; auto.
+  Qed.
+
+  Lemma mkParseTable_complete_wrt_invariant :
+    forall es tbl,
+      unique_action_per_prod es
+      -> table_correct_wrt_entries tbl es
+      -> exists tbl',
+          ParseTable.Equal tbl tbl'
+          /\ mkParseTable es = Some tbl'.
+  Proof.
+    intros es.
+    induction es as [| (xp, la) es]; intros post_tbl Hu Htc.
+    - apply table_correct_wrt_empty_entries_eq_empty_table in Htc.
+      exists empty_table; auto.
+    - pose proof Htc as Htc'.
+      apply correct_post_table_implies_correct_pre_table in Htc.
+      destruct Htc as [pre_tbl Htc].
+      pose proof Htc as Htc''.
+      apply IHes in Htc.
+      destruct Htc as [pre_tbl' [Hpreq Hpremk]].
+      destruct (in_dec pl_pair_eq_dec (plPairOf (xp, la)) (plPairsOf es)).
+      + destruct xp as [(x, gamma) f]; simpl in *.
+        apply in_plPairsOf_ex_in_entries in i.
+        destruct i as [f' Hin].
+        assert (f = f').
+        { unfold unique_action_per_prod in Hu.
+          eapply Hu with (p := (x, gamma)).
+          - left; auto.
+          - right; auto. }
+        subst.
+        exists pre_tbl'; split.
+        * apply invariant_cons_duplicate_invariant_tail in Htc'; auto.
+          -- apply ParseTableFacts.Equal_trans with (m' := pre_tbl); auto.
+             eapply invariant_tables_eq with (es := es); eauto.
+             eapply unique_action_per_prod_tl; eauto.
+        * simpl.
+          rewrite Hpremk.
+          eapply addEntry_duplicate_doesn't_change_table; eauto.
+          eapply equal_preserves_invariant; eauto.
+      + exists (pt_add (lhs xp) la xp pre_tbl'); split.
+        * eapply invariant_not_in_add in Htc''; eauto.
+          -- apply add_preserves_equal with 
+                 (x  := lhs xp)
+                 (la := la)
+                 (xp := xp) in Hpreq; eauto.
+             apply invariant_tables_eq with (tbl := post_tbl) in Htc''; auto.
+             apply ParseTableFacts.Equal_trans with
+                 (m' := pt_add (lhs xp) la xp pre_tbl); auto.
+          -- destruct xp as [(x, gamma) f]; simpl in *.
+             apply not_in_plPairsOf_not_in_entries; auto.
+        * simpl.
+          rewrite Hpremk.
+          eapply addEntry_new_entry_pt_add; eauto.
+          -- eapply equal_preserves_invariant; eauto.
+          -- destruct xp as [(x, gamma) f]; simpl in *.
+             apply not_in_plPairsOf_not_in_entries; auto.
+      + eapply unique_action_per_prod_tl; eauto.
+      + auto.
+  Qed.
+
+  Lemma mkParseTable_complete :
+    forall (es  : list table_entry)
+           (g   : grammar)
+           (tbl : parse_table),
+      unique_productions g
+      -> entries_correct es g
+      -> parse_table_correct tbl g
+      -> exists tbl',
+          ParseTable.Equal tbl tbl'
+          /\ mkParseTable es = Some tbl'.
+  Proof.
+    intros es g tbl Hup Hwf Hpt.
+    apply mkParseTable_complete_wrt_invariant.
+    - eapply unique_productions_unique_action_per_prod; eauto.
+    - eapply invariant_iff_parse_table_correct; eauto.
+  Qed.
   
 End GeneratorProofsFn.
+
